Incremental/Shake/Standard.lean
@@ -51,7 +51,7 @@ def fetch
   | some mm =>
     if hvin : verifyInputs hI ι₀ mm.inputDeps then do
       match ← verifyDeps hI hR tasks ι₀
-          (fun q' _hq => fetch bracket bracket_canReturn ι₀ q') mm.deps with
+          (fun q' _hq => fetch bracket bracket_canReturn ι₀ q') mm.queryDeps with
       | some ⟨hdep⟩ =>
         let value : Value tasks ι₀ q₀ := ⟨mm.value, mm.invariant ι₀
           ((verifyInputs_spec hI ι₀ mm.inputDeps).mp hvin) hdep⟩
